A tiny drop of invariant

Loogle/Trie.lean
@@ -20,7 +20,7 @@ set_option autoImplicit false
 and the internal structure is a tree that branches on the bytes of the string.  -/
 inductive Trie (α : Type) where
   | leaf : Option α → Trie α
-  | path : Option α → ByteArray → Trie α → Trie α
+  | path : Option α → (ps : ByteArray) → 0 < ps.size → Trie α → Trie α
   | node : Option α → ByteArray → Array (Trie α) → Trie α
 
 namespace Trie
@@ -65,42 +65,38 @@ def hasPrefix (s₁ : String) (s₂ : ByteArray) (offset1 : Nat) : Bool :=
   loop 0
 termination_by loop => s₂.size - i
 
+def mkPath (v : Option α) (ps : ByteArray) (t : Trie α) : Trie α :=
+  if h : 0 < ps.size then
+    path v ps h t
+  else
+    t
+
 /-- Insert or update the value at a the given key `s`.  -/
 def upsert (t : Trie α) (s : String) (f : Option α → α) : Trie α :=
   let rec insertEmpty (i : Nat) : Trie α :=
-    if i < s.utf8ByteSize then
-      path none (s.toUTF8.extract i s.utf8ByteSize) (leaf (f .none))
-    else
-      leaf (f .none)
+    mkPath none (s.toUTF8.extract i s.utf8ByteSize) (leaf (f .none))
   let rec loop
     | i, leaf v =>
       if i < s.utf8ByteSize then
-        path v (s.toUTF8.extract i s.utf8ByteSize) (leaf (f .none))
+        mkPath v (s.toUTF8.extract i s.utf8ByteSize) (leaf (f .none))
       else
         leaf (f v)
-    | i, path v ps t' =>
+    | i, path v ps hps t' =>
       if h : i < s.utf8ByteSize then
         let j := commonPrefix s ps i
         if hj : 0 < j then
           -- split common prefix, continue
-          let ps1 := ps.extract 0 j
-          path v ps1 <| loop (i + j) <|
-            if j < ps.size then
-              let ps2 := ps.extract j ps.size
-              path none ps2 t'
-            else
-              t'
+          mkPath v (ps.extract 0 j) <| loop (i + j) <|
+              mkPath none (ps.extract j ps.size) t'
         else
           -- no common prefix, split off first character
           let c := s.getUtf8Byte i h
           let c' := ps.get! 0
           let t := insertEmpty (i + 1)
-          let t'' := if ps.size = 1 then t' else
-            let ps' := ps.extract 1 ps.size
-            path none ps' t'
+          let t'' := mkPath none (ps.extract 1 ps.size) t'
           node v (.mk #[c, c']) #[t, t'']
       else
-        path (f v) ps t'
+        path (f v) ps hps t'
     | i, node v cs ts =>
       if h : i < s.utf8ByteSize then
         let c := s.getUtf8Byte i h
@@ -128,14 +124,12 @@ def find? (t : Trie α) (s : String) : Option α :=
         none
       else
         val
-    | i, path val ps t' =>
+    | i, path val ps _ t' =>
       if i < s.utf8ByteSize then
-        if 0 < ps.size then
-          if hasPrefix s ps i then
-            loop (i + ps.size) t'
-          else
-            none
-        else none -- should be dead code
+        if hasPrefix s ps i then
+          loop (i + ps.size) t'
+        else
+          none
       else
         val
     | i, node val cs ts =>
@@ -157,7 +151,7 @@ def values (t : Trie α) : Array α := go t |>.run #[] |>.2
       | leaf a? => do
         if let some a := a? then
           modify (·.push a)
-      | path a? _ t' => do
+      | path a? _ _ t' => do
         if let some a := a? then
           modify (·.push a)
         go t'
@@ -174,13 +168,10 @@ def findPrefix (t : Trie α) (pre : String) : Array α := go t 0
         let c := pre.getUtf8Byte i h
         match t with
         | leaf _val => .empty
-        | path _val ps t' =>
-          if 0 < ps.size then
-            if hasPrefix pre ps i
-            then go t' (i + ps.size)
-            else .empty
-          else
-            .empty -- should be an invariant
+        | path _val ps _ t' =>
+          if hasPrefix pre ps i
+          then go t' (i + ps.size)
+          else .empty
         | node _val cs ts =>
           match cs.findIdx? (· == c) with
           | none   => .empty
@@ -195,7 +186,7 @@ def findPrefix (t : Trie α) (pre : String) : Array α := go t 0
 open Lean in
 private partial def toStringAux {α : Type} : Trie α → List Format
   | leaf _ => []
-  | path _ ps t =>
+  | path _ ps _ t =>
     [ format (repr ps.data), Format.group $ Format.nest 4 $ flip Format.joinSep Format.line $ toStringAux t ]
   | node _ cs ts =>
     List.join $ List.zipWith (fun c t =>
